FTLR - Case Load

theories/ftlr/Load.v
@@ -11,20 +11,22 @@ Section fundamental.
           {nainv: logrel_na_invs Σ}
           `{MachineParameters}.
 
-  Notation D := ((leibnizO Word) -n> iPropO Σ).
-  Notation R := ((leibnizO Reg) -n> iPropO Σ).
-  Implicit Types w : (leibnizO Word).
+  Notation D := ((leibnizO LWord) -n> iPropO Σ).
+  Notation R := ((leibnizO LReg) -n> iPropO Σ).
+  Implicit Types lw : (leibnizO LWord).
   Implicit Types interp : (D).
 
   (* The necessary resources to close the region again, except for the points to predicate, which we will store separately
    The boolean bl can be used to keep track of whether or not we have applied a wp lemma *)
-  Definition region_open_resources (P : D) (w : Word) (a pc_a : Addr) (f:bool) : iProp Σ :=
-    ((if f then ▷ P w else P w) ∗ read_cond P interp ∗ ((▷ ∃ w0, a ↦ₐ w0 ∗ P w0) ={⊤ ∖ ↑logN.@pc_a ∖ ↑logN.@a,⊤ ∖ ↑logN.@pc_a}=∗ emp))%I.
+  Definition region_open_resources (P : D) (lw : LWord) (la pc_la : LAddr) (f:bool) : iProp Σ :=
+    ((if f then ▷ P lw else P lw)
+       ∗ read_cond P interp
+       ∗ ((▷ ∃ lw0, la ↦ₐ lw0 ∗ P lw0) ={⊤ ∖ ↑logN.@pc_la ∖ ↑logN.@la,⊤ ∖ ↑logN.@pc_la}=∗ emp))%I.
 
-  Lemma load_inr_eq {regs r p0 b0 e0 a0 p1 b1 e1 a1}:
-    reg_allows_load regs r p0 b0 e0 a0 →
-    read_reg_inr regs r p1 b1 e1 a1 →
-    p0 = p1 ∧ b0 = b1 ∧ e0 = e1 ∧ a0 = a1.
+  Lemma load_inr_eq {regs r p0 b0 e0 a0 v0 p1 b1 e1 a1 v1}:
+    reg_allows_load regs r p0 b0 e0 a0 v0 →
+    read_reg_inr regs r p1 b1 e1 a1 v1 →
+    p0 = p1 ∧ b0 = b1 ∧ e0 = e1 ∧ a0 = a1 /\ v0 = v1.
   Proof.
       intros Hrar H3.
       pose (Hrar' := Hrar).
@@ -33,44 +35,49 @@ Section fundamental.
 
 
   (* Description of what the resources are supposed to look like after opening the region if we need to, but before closing the region up again*)
-  Definition allow_load_res r (regs : Reg) pc_a a p b e (P : D) :=
-    (⌜read_reg_inr regs r p b e a⌝ ∗
-    if decide (reg_allows_load regs r p b e a ∧ a ≠ pc_a ) then
-         |={⊤ ∖ ↑logN.@pc_a,⊤ ∖ ↑logN.@pc_a ∖ ↑logN.@a}=> ∃ w, a ↦ₐ w ∗ region_open_resources P w a pc_a true ∗ ▷ interp w
+  Definition allow_load_res (lregs : LReg) (r : RegName) pc_a pca_v p b e a v (P : D) :=
+    (⌜read_reg_inr lregs r p b e a v⌝ ∗
+    if decide (reg_allows_load lregs r p b e a v ∧ (a,v) ≠ (pc_a,pca_v))
+    then
+      |={⊤ ∖ ↑logN.@(pc_a, pca_v),⊤ ∖ ↑logN.@(pc_a, pca_v) ∖ ↑logN.@(a,v)}=>
+        ∃ lw, (a, v) ↦ₐ lw ∗ region_open_resources P lw (a,v) (pc_a, pca_v) true ∗ ▷ interp lw
      else True)%I.
 
 
-  Definition allow_load_mem r (regs : Reg) (pc_a : Addr) (pc_w : Word) (mem : gmap Addr Word) (a : Addr) p b e (P:D) (f:bool) :=
-    (⌜read_reg_inr regs r p b e a⌝ ∗
-    if decide (reg_allows_load regs r p b e a ∧ a ≠ pc_a) then
-         ∃ (w : Word), ⌜mem = <[a:=w]> (<[pc_a:=pc_w]> ∅)⌝ ∗
-            (region_open_resources P w a pc_a f) ∗ if f then ▷ interp w else interp w
-    else  ⌜mem = <[pc_a:=pc_w]> ∅⌝)%I.
+  Definition allow_load_mem (lregs : LReg) (r : RegName)
+    (pc_a : Addr) (pca_v : Version) (pc_lw : LWord)
+    (lmem : LMem) p b e (a : Addr) (v : Version) (P:D) (f:bool) :=
+    (⌜read_reg_inr lregs r p b e a v⌝ ∗
+    if decide (reg_allows_load lregs r p b e a v ∧ (a,v) ≠ (pc_a,pca_v) ) then
+         ∃ (lw : LWord), ⌜lmem = <[(a,v):=lw]> (<[(pc_a, pca_v):=pc_lw]> ∅)⌝ ∗
+            (region_open_resources P lw (a,v) (pc_a, pca_v) f) ∗ if f then ▷ interp lw else interp lw
+    else  ⌜lmem = <[(pc_a, pca_v):=pc_lw]> ∅⌝)%I.
 
   Lemma create_load_res:
-    ∀ (r : leibnizO Reg) (p : Perm)
-      (b e a : Addr) (src : RegName) (p0 : Perm)
-      (b0 e0 a0 : Addr),
-      read_reg_inr (<[PC:=WCap p b e a]> r) src p0 b0 e0 a0
-      → (∀ (r1 : RegName) v, ⌜r1 ≠ PC⌝ → ⌜r !! r1 = Some v⌝ → (fixpoint interp1) v)
-          -∗ ∃ P, allow_load_res src (<[PC:=WCap p b e a]> r) a a0 p0 b0 e0 P.
+    ∀ (lregs : leibnizO LReg) (p : Perm)
+      (b e a : Addr) (v : Version) (src : RegName) (p0 : Perm)
+      (b0 e0 a0 : Addr) (v0 : Version),
+      read_reg_inr (<[PC:=LCap p b e a v]> lregs) src p0 b0 e0 a0 v0
+      → (∀ (r1 : RegName) lv, ⌜r1 ≠ PC⌝ → ⌜lregs !! r1 = Some lv⌝ → (fixpoint interp1) lv)
+          -∗ ∃ P, allow_load_res (<[PC:=LCap p b e a v]> lregs) src a v p0 b0 e0 a0 v0 P.
   Proof.
-    intros r p b e a src p0 b0 e0 a0 HVsrc.
+    intros lregs p b e a v src p0 b0 e0 a0 v0 HVsrc.
     iIntros "#Hreg". rewrite /allow_load_res.
-    (* do 5 (iApply sep_exist_r; iExists _). *) (* do 3 (iExists _). *) iFrame "%".
-    case_decide as Hdec. 1: destruct Hdec as [Hallows Haeq].
+    iFrame "%".
+    case_decide as Hdec. 1: destruct Hdec as [Hallows Hlaeq].
     -  destruct Hallows as [Hrinr [Hra Hwb] ].
          apply andb_prop in Hwb as [Hle Hge].
 
          (* Unlike in the old proof, we now go the other way around, and prove that the source register could not have been the PC, since both addresses differ. This saves us some cases.*)
-         assert (src ≠ PC) as n. refine (addr_ne_reg_ne Hrinr _ Haeq). by rewrite lookup_insert.
+         assert (src ≠ PC) as n.
+         refine (laddr_ne_reg_ne Hrinr _ Hlaeq). by rewrite lookup_insert.
 
          rewrite lookup_insert_ne in Hrinr; last by congruence.
          iDestruct ("Hreg" $! src _ n Hrinr) as "Hvsrc".
          iDestruct (read_allowed_inv _ a0 with "Hvsrc") as (P) "[Hinv [Hconds _] ]"; auto;
            first (split; [by apply Z.leb_le | by apply Z.ltb_lt]).
          iExists P.
-         iMod (inv_acc (⊤ ∖ ↑logN.@a) with "Hinv") as "[Hrefinv Hcls]";[solve_ndisj|].
+         iMod (inv_acc (⊤ ∖ ↑logN.@(a,v)) with "Hinv") as "[Hrefinv Hcls]";[solve_ndisj|].
          rewrite /interp_ref_inv /=. iDestruct "Hrefinv" as (w) "[>Ha HP]".
          iExists w.
          iAssert (▷ interp w)%I as "#Hw".
@@ -79,34 +86,36 @@ Section fundamental.
     - iExists (λne _, True%I). done.
   Qed.
 
-  (* Definition allow_load_mask (a a0 : Addr) : namespace := *)
-  (*   if decide (a = a0) then ⊤ ∖ ↑logN.@a else ⊤ ∖ ↑logN.@a ∖ ↑logN.@a0.  *)
-
   Lemma load_res_implies_mem_map:
-    ∀ (r : leibnizO Reg)
-       (a a0 : Addr) (w : Word) (src : RegName) p1 b1 e1 (P:D),
-      allow_load_res src r a a0 p1 b1 e1 P
-      -∗ a ↦ₐ w
-      ={⊤ ∖ ↑logN.@a,if decide (reg_allows_load r src p1 b1 e1 a0 ∧ a0 ≠ a) then ⊤ ∖ ↑logN.@a ∖ ↑logN.@a0 else ⊤ ∖ ↑logN.@a}=∗ ∃ mem0 : gmap Addr Word,
-          allow_load_mem src r a w mem0 a0 p1 b1 e1 P true
-            ∗ ▷ ([∗ map] a0↦w ∈ mem0, a0 ↦ₐ w).
+    ∀ (lregs : leibnizO LReg)
+       (a a0 : Addr) (v v0 : Version) (lw : LWord) (src : RegName) p1 b1 e1 (P:D),
+      allow_load_res lregs src a v p1 b1 e1 a0 v0 P
+      -∗ (a, v) ↦ₐ lw
+      ={⊤ ∖ ↑logN.@(a,v),
+        if decide (reg_allows_load lregs src p1 b1 e1 a0 v0 ∧ (a0,v0) ≠ (a,v))
+        then ⊤ ∖ ↑logN.@(a,v) ∖ ↑logN.@(a0,v0)
+        else ⊤ ∖ ↑logN.@(a,v)}=∗
+         ∃ lmem : LMem,
+           allow_load_mem lregs src a v lw lmem p1 b1 e1 a0 v0 P true
+             ∗ ▷ ([∗ map] la↦lw ∈ lmem, la ↦ₐ lw).
   Proof.
-    intros r a a0 w src p1 b1 e1 P.
+    intros lregs a a0 v v0 w src p1 b1 e1 P.
     iIntros "HLoadRes Ha".
     iDestruct "HLoadRes" as "[% HLoadRes]".
 
-    case_decide as Hdec. 1: destruct Hdec as [ Hallows Haeq ].
+    case_decide as Hdec. 1: destruct Hdec as [ Hallows Hlaeq ].
     -  pose(Hallows' := Hallows). destruct Hallows' as [Hrinr [Hra Hwb] ].
-       iMod "HLoadRes" as (w0) "[Ha0 [HLoadRest #Hval] ]".
+       iMod "HLoadRes" as (lw0) "[Ha0 [HLoadRest #Hval] ]".
        iExists _.
        iSplitL "HLoadRest".
        + iSplitR; first auto.
 
          case_decide as Hdec1.
-         2: apply not_and_r in Hdec1 as [|]; by exfalso.
-         iExists w0. iSplitR; auto.
+         2: { apply not_and_r in Hdec1 as [| Hdec1] ; by exfalso. }
+         iExists lw0. iSplitR; auto.
        + iModIntro. iNext.
-         rewrite memMap_resource_2ne; auto; iFrame.
+         rewrite memMap_resource_2ne; first iFrame.
+         intro ; simplify_eq.
     - rewrite /read_reg_inr in H0.
       iExists _.
       iSplitL "HLoadRes".
@@ -116,63 +125,73 @@ Section fundamental.
   Qed.
 
   Lemma mem_map_implies_pure_conds:
-    ∀ (r : leibnizO Reg)
-       (a a0 : Addr) (w : Word) (src : RegName)
-      (mem0 : gmap Addr Word) p b e P f,
-        allow_load_mem src r a w mem0 a0 p b e P f
-        -∗ ⌜mem0 !! a = Some w⌝
-          ∗ ⌜allow_load_map_or_true src r mem0⌝.
+    ∀ (lregs : leibnizO LReg)
+       (a a0 : Addr) (v v0 : Version) (lw : LWord) (src : RegName)
+       (lmem : LMem) p b e P f,
+        allow_load_mem lregs src a v lw lmem p b e a0 v0 P f
+        -∗ ⌜lmem !! (a,v) = Some lw⌝
+          ∗ ⌜allow_load_map_or_true src lregs lmem⌝.
   Proof.
-    iIntros (r a a0 w src mem0 p b e P f) "HLoadMem".
+    iIntros (lregs a a0 v v0 lw src lmem p b e P f) "HLoadMem".
     iDestruct "HLoadMem" as "[% HLoadRes]".
-    case_decide as Hdec. 1: destruct Hdec as [ Hallows Haeq ].
+    case_decide as Hdec. 1: destruct Hdec as [ Hallows Hlaeq ].
     -  pose(Hallows' := Hallows). destruct Hallows' as [Hrinr [Hra Hwb] ].
        (* case_decide as Haeq. *)
-       iDestruct "HLoadRes" as (w0) "[% _]".
+       iDestruct "HLoadRes" as (lw0) "[% _]".
        iSplitR. rewrite H1 lookup_insert_ne; auto. by rewrite lookup_insert.
-       iExists p,b,e,a0. iSplitR; auto.
+       iExists p,b,e,a0,v0. iSplitR; auto.
        case_decide; last by exfalso.
-       iExists w0. rewrite H1.
+       iExists lw0. rewrite H1.
          by rewrite lookup_insert.
     - iDestruct "HLoadRes" as "->".
       iSplitR. by rewrite lookup_insert.
-      iExists p,b,e,a0. iSplitR; auto.
+      iExists p,b,e,a0,v0. iSplitR; auto.
       case_decide as Hdec1; last by done.
       apply not_and_r in Hdec as [| <-%dec_stable]; first by exfalso.
-      iExists w. by rewrite lookup_insert.
+      iExists lw.
+      by rewrite lookup_insert.
   Qed.
 
   Lemma allow_load_mem_later:
-    ∀ (r : leibnizO Reg) (p : Perm)
-      (b e a a0 : Addr) (w : Word) (src : RegName)
-      (mem0 : gmap Addr Word) p0 b0 e0 P,
-      allow_load_mem src r a w mem0 a0 p0 b0 e0 P true
-      -∗ ▷ allow_load_mem src r a w mem0 a0 p0 b0 e0 P false.
+    ∀ (lregs : leibnizO LReg)
+      (p : Perm) (b e a a0 : Addr) (v v0 : Version)
+      (lw : LWord) (src : RegName)
+      (lmem : LMem) p0 b0 e0 P,
+      allow_load_mem lregs src a v lw lmem p0 b0 e0 a0 v0 P true
+      -∗ ▷ allow_load_mem lregs src a v lw lmem p0 b0 e0 a0 v0 P false.
   Proof.
-    iIntros (r p b e a a0 w src mem0 p0 b0 e0 P) "HLoadMem".
+    iIntros (lregs p b e a a0 v v0 lw src lmem p0 b0 e0 P) "HLoadMem".
     iDestruct "HLoadMem" as "[% HLoadMem]".
     rewrite !/allow_load_mem /=. iSplit;[auto|].
-    destruct (decide (reg_allows_load r src p0 b0 e0 a0 ∧ a0 ≠ a)).
-    - iApply later_exist_2. iDestruct "HLoadMem" as (w0) "(?&HP&?)".
-      iExists w0. iNext. iDestruct "HP" as "(?&?&?)". iFrame.
+    destruct (decide (reg_allows_load lregs src p0 b0 e0 a0 v0 ∧ (a0,v0) ≠ (a,v))).
+    - iApply later_exist_2. iDestruct "HLoadMem" as (lw0) "(?&HP&?)".
+      iExists lw0. iNext. iDestruct "HP" as "(?&?&?)". iFrame.
     - iNext. iFrame.
   Qed.
 
-  Instance if_Persistent p b e a r src p0 b0 e0 a0 loadv : Persistent (if decide (reg_allows_load (<[PC:=WCap p b e a]> r) src p0 b0 e0 a0 ∧ a0 ≠ a) then interp loadv else emp)%I.
-  Proof. intros. destruct (decide (reg_allows_load (<[PC:=WCap p b e a]> r) src p0 b0 e0 a0 ∧ a0 ≠ a));apply _. Qed.
+  Instance if_Persistent p b e a v lregs src p0 b0 e0 a0 v0 loadv :
+    Persistent (if decide (reg_allows_load (<[PC:=LCap p b e a v]> lregs) src p0 b0 e0 a0 v0 ∧ (a0, v0) ≠ (a,v))
+                then interp loadv
+                else emp)%I.
+  Proof. intros. destruct (decide (reg_allows_load (<[PC:=LCap p b e a v]> lregs) src p0 b0 e0 a0 v0 ∧ (a0, v0) ≠ (a,v)));apply _. Qed.
 
   Lemma mem_map_recover_res:
-    ∀ (r : leibnizO Reg)
-       (a : Addr) (w : Word) (src : RegName) p0
-       (b0 e0 a0 : Addr) (mem0 : gmap Addr Word) loadv P,
-      mem0 !! a0 = Some loadv
-      -> reg_allows_load r src p0 b0 e0 a0
-      → allow_load_mem src r a w mem0 a0 p0 b0 e0 P false
-        -∗ ([∗ map] a0↦w ∈ mem0, a0 ↦ₐ w)
-        ={if decide (reg_allows_load r src p0 b0 e0 a0 ∧ a0 ≠ a) then ⊤ ∖ ↑logN.@a ∖ ↑logN.@a0 else ⊤ ∖ ↑logN.@a,⊤ ∖ ↑logN.@a}=∗ a ↦ₐ w
-                  ∗ if decide (reg_allows_load r src p0 b0 e0 a0 ∧ a0 ≠ a) then interp loadv else emp.
+    ∀ (lregs : leibnizO LReg)
+       (a : Addr) (v : Version) (lw : LWord) (src : RegName) p0
+       (b0 e0 a0 : Addr) (v0 : Version) (lmem : LMem) loadv P,
+      lmem !! (a0, v0) = Some loadv
+      -> reg_allows_load lregs src p0 b0 e0 a0 v0
+      → allow_load_mem lregs src  a v lw lmem p0 b0 e0 a0 v0 P false
+        -∗ ([∗ map] la↦lw ∈ lmem, la ↦ₐ lw)
+        ={if decide (reg_allows_load lregs src p0 b0 e0 a0 v0 ∧ (a0, v0) ≠ (a,v))
+          then ⊤ ∖ ↑logN.@(a,v) ∖ ↑logN.@(a0,v0)
+          else ⊤ ∖ ↑logN.@(a,v),⊤ ∖ ↑logN.@(a,v)}=∗
+           (a,v) ↦ₐ lw
+           ∗ if decide (reg_allows_load lregs src p0 b0 e0 a0 v0 ∧ (a0, v0) ≠ (a,v))
+           then interp loadv
+           else emp.
   Proof.
-    intros r a w src p0 b0 e0 a0 mem0 loadv P Hloadv Hrar.
+    intros lregs a v lw src p0 b0 e0 a0 v0 lmem loadv P Hloadv Hrar.
     iIntros "HLoadMem Hmem".
     iDestruct "HLoadMem" as "[% HLoadRes]".
     (* destruct (load_inr_eq Hrar H0) as (<- & <- &<- &<- &<-). *)
@@ -189,9 +208,10 @@ Section fundamental.
   Qed.
 
 
-  Lemma load_case (r : leibnizO Reg) (p : Perm)
-        (b e a : Addr) (w : Word) (dst src : RegName) (P : D):
-    ftlr_instr r p b e a w (Load dst src) P.
+  Lemma load_case (lregs : leibnizO LReg)
+    (p : Perm) (b e a : Addr) (v : Version)
+    (lw : LWord) (dst src : RegName) (P : D):
+    ftlr_instr lregs p b e a v lw (Load dst src) P.
   Proof.
     intros Hp Hsome i Hbae Hi.
     iIntros "#IH #Hinv #Hinva #Hreg #[Hread Hwrite] Hown Ha HP Hcls HPC Hmap".
@@ -200,7 +220,7 @@ Section fundamental.
       [apply lookup_insert|rewrite delete_insert_delete;iFrame|]. simpl.
 
     (* To read out PC's name later, and needed when calling wp_load *)
-    assert(∀ x : RegName, is_Some (<[PC:=WCap p b e a]> r !! x)) as Hsome'.
+    assert(∀ x : RegName, is_Some (<[PC:=LCap p b e a v]> lregs !! x)) as Hsome'.
     {
       intros. destruct (decide (x = PC)).
       rewrite e0 lookup_insert; unfold is_Some. by eexists.
@@ -208,12 +228,13 @@ Section fundamental.
     }
 
     (* Initializing the names for the values of Hsrc now, to instantiate the existentials in step 1 *)
-    assert (∃ p0 b0 e0 a0, read_reg_inr (<[PC:=WCap p b e a]> r) src p0 b0 e0 a0) as [p0 [b0 [e0 [a0 HVsrc] ] ] ].
+    assert (∃ p0 b0 e0 a0 v0, read_reg_inr (<[PC:=LCap p b e a v]> lregs) src p0 b0 e0 a0 v0)
+      as (p0 & b0 & e0 & a0 & v0 & HVsrc).
     {
       specialize Hsome' with src as Hsrc.
       destruct Hsrc as [wsrc Hsomesrc].
       unfold read_reg_inr. rewrite Hsomesrc.
-      destruct wsrc as [|[ p0 b0 e0 a0|] | ]; try done.
+      destruct wsrc as [|[ p0 b0 e0 a0 v0|] | ]; try done.
       by repeat eexists.
     }
 
@@ -222,7 +243,7 @@ Section fundamental.
     iDestruct (create_load_res with "Hreg") as (P') "HLoadRes"; eauto.
 
     (* Step2: derive the concrete map of memory we need, and any spatial predicates holding over it *)
-    iMod (load_res_implies_mem_map with "HLoadRes Ha") as (mem0) "[HLoadMem HLoadRest]".
+    iMod (load_res_implies_mem_map with "HLoadRes Ha") as (lmem) "[HLoadMem HLoadRest]".
 
     (* Step 3:  derive the non-spatial conditions over the memory map*)
     iDestruct (mem_map_implies_pure_conds with "HLoadMem") as %(HReadPC & HLoadAP); auto.
@@ -240,20 +261,19 @@ Section fundamental.
     (* Infer that if P holds at w, then w must be valid (read condition) *)
     iDestruct ("Hread" with "HP") as "#Hw".
 
-    destruct HSpec as [* ? ? Hincr|].
-    { apply incrementPC_Some_inv in Hincr.
-      destruct Hincr as (?&?&?&?&?&?&?&?).
+    destruct HSpec as [* HregLoad Hmem Hincr|].
+    { apply incrementLPC_Some_inv in Hincr as (p''&b''&e''&a''&?& v'' & HPC & Z & Hregs') .
       iApply wp_pure_step_later; auto.
-      specialize (load_inr_eq H0 HVsrc) as (-> & -> & -> & ->).
+      specialize (load_inr_eq HregLoad HVsrc) as (-> & -> & -> & -> & ->).
       rewrite /allow_load_res.
       (* Step 5: return all the resources we had in order to close the second location in the region, in the cases where we need to *)
       iMod (mem_map_recover_res with "HLoadMem Hmem") as "[Ha #Hinterp]";[eauto|auto|iModIntro].
-      iMod ("Hcls" with "[Ha HP]");[iExists w;iFrame|iModIntro].
+      iMod ("Hcls" with "[Ha HP]");[iExists lw;iFrame|iModIntro].
 
       (* Exceptional success case: we do not apply the induction hypothesis in case we have a faulty PC *)
-      destruct (decide (x = RX ∨ x = RWX)).
+      destruct (decide (p'' = RX ∨ p'' = RWX)).
       2 : {
-        assert (x ≠ RX ∧ x ≠ RWX). split; by auto.
+        assert (p'' ≠ RX ∧ p'' ≠ RWX). split; by auto.
         iDestruct ((big_sepM_delete _ _ PC) with "Hmap") as "[HPC Hmap]".
         { subst. by rewrite lookup_insert. }
         iNext; iIntros "_".
@@ -267,20 +287,22 @@ Section fundamental.
 
       iNext; iIntros "_".
       iApply ("IH" $! regs' with "[%] [Hinterp] [Hmap] [$Hown]").
-      { cbn. intros. subst regs'.
+      { cbn. intros rx. subst regs'.
         rewrite lookup_insert_is_Some.
-        destruct (decide (PC = x4)); [ auto | right; split; auto].
+        destruct (decide (PC = rx)); [ auto | right; split; auto].
         rewrite lookup_insert_is_Some.
-        destruct (decide (dst = x4)); [ auto | right; split; auto]. }
+        destruct (decide (dst = rx)); [ auto | right; split; auto]. }
       (* Prove in the general case that the value relation holds for the register that was loaded to - unless it was the PC.*)
-       { iIntros (ri v Hri Hvs).
+       { iIntros (ri ? Hri Hvs).
         subst regs'.
         rewrite lookup_insert_ne in Hvs; auto.
         destruct (decide (ri = dst)).
         { subst ri.
-          rewrite lookup_insert in Hvs; auto. inversion Hvs.
-          destruct (decide (a = a0)).
-          - simplify_eq. iFrame "Hw".
+          rewrite lookup_insert_ne // lookup_insert in HPC; simplify_eq.
+          rewrite lookup_insert in Hvs; auto; inversion Hvs; simplify_eq.
+          destruct (decide ((a0, v0) = (a'', v''))).
+          - simplify_eq.
+            iFrame "Hw".
           - iClear "HLoadRes Hwrite". rewrite decide_True. iFrame "#". auto.
         }
         { repeat (rewrite lookup_insert_ne in Hvs); auto.
@@ -290,7 +312,7 @@ Section fundamental.
        { iModIntro.
          destruct (decide (PC = dst)); simplify_eq.
          - simplify_map_eq. rewrite (fixpoint_interp1_eq).
-           destruct (decide (a = a0)).
+           destruct (decide ((a0, v0) = (a, v))).
            + simplify_map_eq.
            + iClear "HLoadRes Hwrite". rewrite decide_True;auto.
              rewrite !fixpoint_interp1_eq.
@@ -302,18 +324,18 @@ Section fundamental.
        }
     }
     { rewrite /allow_load_res /allow_load_mem.
-      destruct (decide (reg_allows_load (<[PC:=WCap p b e a]> r) src p0 b0 e0 a0 ∧ a0 ≠ a)).
+      destruct (decide (reg_allows_load (<[PC:=LCap p b e a v]> lregs) src p0 b0 e0 a0 v0 ∧ (a0, v0) ≠ (a, v))).
       - iDestruct "HLoadMem" as "(_&H)".
-        iDestruct "H" as (w') "(->&Hres&Hinterp)". rewrite /region_open_resources.
+        iDestruct "H" as (lw') "(->&Hres&Hinterp)". rewrite /region_open_resources.
         destruct a1. rewrite memMap_resource_2ne; last auto.
         iDestruct "Hmem" as "[Ha0 Ha]". iDestruct "Hres" as "(HP' & Hread' & Hcls')".
-        iMod ("Hcls'" with "[HP' Ha0]");[iExists w';iFrame|iModIntro].
-        iMod ("Hcls" with "[Ha HP]");[iExists w;iFrame|iModIntro].
+        iMod ("Hcls'" with "[HP' Ha0]");[iExists lw';iFrame|iModIntro].
+        iMod ("Hcls" with "[Ha HP]");[iExists lw;iFrame|iModIntro].
         iApply wp_pure_step_later; auto.
         iNext; iIntros "_".
         iApply wp_value; auto. iIntros; discriminate.
       - iModIntro. iDestruct "HLoadMem" as "(_&->)". rewrite -memMap_resource_1.
-        iMod ("Hcls" with "[Hmem HP]");[iExists w;iFrame|iModIntro].
+        iMod ("Hcls" with "[Hmem HP]");[iExists lw;iFrame|iModIntro].
         iApply wp_pure_step_later; auto.
         iNext; iIntros "_".
         iApply wp_value; auto. iIntros; discriminate.
